compiler/backend/data_to_wordScript.sml
@@ -2477,6 +2477,7 @@ Definition assign_def:
     | MemOp (CopyByte alloc_new) => assign_CopyByte c secn l dest names args
     | MemOp RefArray => arg2 args (assign_RefArray c secn l dest names) (Skip,l)
     | BlockOp (BoolTest test) => arg2 args (assign_BoolTest l dest test) (Skip,l)
+    | BlockOp PtrEqual => arg2 args (assign_BoolTest l dest Equal) (Skip,l)
     | BlockOp BoolNot => arg1 args (assign_BoolNot l dest) (Skip,l)
     | WordOp (WordTest ws test) => arg2 args (assign_WordTest l dest test) (Skip,l)
     | BlockOp (FromList tag) => arg2 args (assign_FromList c secn l dest names tag) (Skip,l)
